llvm.checker: rewrite a lot, simple subet

cogent/llvm/checker/coq/Compiler.v
@@ -4,7 +4,7 @@ From ExtLib Require Import Structures.Monads Structures.Functor Structures.Reduc
 From RecordUpdate Require Import RecordSet.
 From Vellvm Require Import LLVMAst Util Utils.Error.
 
-From Checker Require Import Cogent Types Utils.ErrorWithState Utils.Instances.
+From Checker Require Import Cogent Types Utils.ErrorWithState Utils.Instances Utils.Codegen.
 
 Import ListNotations.
 Import RecordSetNotations.
@@ -14,34 +14,34 @@ Local Open Scope monad_scope.
 
 Section Compiler.
 
-  Definition CodegenValue : Type := texp typ.
+  Definition segment : Type := texp typ * block_id * list (block typ).
+
+  (* Definition CodegenValue : Type := texp typ.
+   
+
+  (* use similar strategy to helix *)
+  Definition segment : Type := block_id * list (block typ).
 
   Record CodegenState : Type := mk_state {
-    entry : block typ
-  ; blocks : list (block typ)
+    fresh_void : Z
   ; fresh_anon : Z
   ; fresh_block : Z
   ; vars : list (texp typ)
   }.
 
-  Instance etaCodegenState : Settable _ := settable! mk_state <
-    entry
-  ; blocks
+  Global Instance etaCodegenState : Settable _ := settable! mk_state <
+    fresh_void
   ; fresh_anon
   ; fresh_block
   ; vars
   >.
 
-  Instance etaBlock : Settable _ := settable! (@mk_block typ) <blk_id;blk_phis; blk_code; blk_term; blk_comments>.
+  Global Instance etaBlock : Settable _ := settable! (@mk_block typ) <blk_id;blk_phis; blk_code; blk_term; blk_comments>.
 
   Definition empty_block (n : block_id) : block typ :=
     mk_block n [] [] TERM_Ret_void None.
 
   Definition cerr := errS CodegenState.
-
-  Definition current_block : cerr block_id :=
-    s <- get ;;
-    ret (blk_id (hd (entry s) (blocks s))).
 
   Definition update_block (f : block typ -> block typ) (s : CodegenState) : CodegenState :=
     match blocks s with
@@ -97,9 +97,9 @@ Section Compiler.
     set_vars (var :: vars s) ;;
     res <- action ;;
     set_vars (vars s) ;;
-    ret res.
+    ret res. *)
 
-  Definition int32 (n : int) : texp typ := (TYPE_I 32, EXP_Integer n).
+  (* Definition int32 (n : int) : texp typ := (TYPE_I 32, EXP_Integer n). *)
 
 
   Definition compile_prim_op (o : prim_op) : (exp typ -> exp typ -> exp typ) * typ :=
@@ -122,12 +122,12 @@ Section Compiler.
     | TRecord ts s => 
         let t' := TYPE_Struct (map (fun '(_, (f, _)) => compile_type f) ts) in
           match s with Boxed => TYPE_Pointer t' | Unboxed => t' end
-    | TUnit => TYPE_I 8
+    | TUnit => TYPE_I 2
     end.
 
-  Fixpoint compile_expr (e : expr) : cerr CodegenValue :=
+  Fixpoint compile_expr (e : expr) (next_blk : block_id) : cerr segment :=
     (* define some nested functions that are mutually recursive with compile_expr *)
-    let fix load_member e f : cerr (CodegenValue * CodegenValue) :=
+    (* let fix load_member e f : cerr (CodegenValue * CodegenValue) :=
       e' <- compile_expr e ;;
       f' <- match field_type (fst e') f with
       | UnboxField t => instr t (INSTR_Op (OP_ExtractValue e' [Z.of_nat f]))
@@ -137,33 +137,38 @@ Section Compiler.
           instr t (INSTR_Load false t p None)
       | Invalid => raise "invalid member access"
       end ;;
-      ret (e', f') in
+      ret (e', f') in *)
     match e with
     | Prim op os =>
         match os with
-        | [oa; ob] => 
+        | [a; b] => 
             let (op', rt) := compile_prim_op op in
-              va <- snd <$> compile_expr oa ;;
-              vb <- snd <$> compile_expr ob ;;
-              instr rt (INSTR_Op (op' va vb)) 
+              prim_blk <- incBlockNamed "Prim" ;;
+              '((_, b_val), b_blk, b_blks) <- compile_expr b prim_blk ;;
+              '((_, a_val), a_blk, a_blks) <- compile_expr a b_blk ;;
+              new_local <- incLocal ;;
+              ret ((rt, EXP_Ident (ID_Local (new_local))), a_blk, a_blks ++ b_blks ++ [code_block prim_blk next_blk [(IId new_local, INSTR_Op (op' a_val b_val))]])
         | _ => raise "wrong number of primitive arguments"
         end
-    | Lit l => ret match l with
+    | Lit l => ret (match l with
       | LBool b => (TYPE_I 1, EXP_Integer (if b then 1 else 0))
       | LU8 w => (TYPE_I 8, EXP_Integer w)
       | LU16 w => (TYPE_I 16, EXP_Integer w)
       | LU32 w => (TYPE_I 32, EXP_Integer w)
       | LU64 w => (TYPE_I 64, EXP_Integer w)
-      end
-    | Var i =>
-        s <- get ;;
-        match (nth_error (vars s) i) with
-        | Some v => ret v
-        | None => raise "unknown variable"
-        end
-    | Let e b => compile_expr e >>= flip bind (compile_expr b)
-    | Unit => ret (TYPE_I 2, EXP_Integer 0)
-    | If c t e =>
+      end, next_blk, [])
+    | Var i => 
+        v <- getStateVar "unknown variable" i ;;
+        ret (v, next_blk, [])
+    | Let e b =>
+        let_blk <- incBlockNamed "Let" ;;
+        '(e', e_blk, e_blks) <- compile_expr e let_blk ;;
+        addVars [e'] ;;
+        '(b', b_blk, b_blks) <- compile_expr b next_blk ;;
+        dropVars 1 ;;
+        ret (b', e_blk, e_blks ++ [code_block let_blk b_blk []] ++ b_blks)
+    | Unit => ret ((TYPE_I 2, EXP_Integer 0), next_blk, [])
+    (* | If c t e =>
         c' <- compile_expr c ;;
         '(br_true, br_false, br_exit) <- branch_blocks ;;
         term (TERM_Br c' br_true br_false) ;;
@@ -208,23 +213,22 @@ Section Compiler.
     | App f a =>
         a' <- compile_expr a ;;
         f' <- compile_expr f ;;
-        instr (return_type (deref_type (fst f'))) (INSTR_Call f' [a'])
+        instr (return_type (deref_type (fst f'))) (INSTR_Call f' [a']) *)
     end.
 
-  (* eventually will need to share this state between functions *)
-  Definition start_state (t : typ) : CodegenState := {|
-    entry := empty_block (Name "entry_0")
-  ; blocks := []
-  ; fresh_anon := 0
-  ; fresh_block := 0
-  ; vars := [(t, EXP_Ident (ID_Local (Name "a_0")))]
-  |}.
+  (* Definition build_expr (p : expr) (t : type) : err CodegenState :=
+    execErrS (v <- compile_expr p ;; term (TERM_Ret v)) (start_state (compile_type t)). *)
 
-  Definition build_expr (p : expr) (t : type) : err CodegenState :=
-    execErrS (v <- compile_expr p ;; term (TERM_Ret v)) (start_state (compile_type t)).
-
-  Definition compile_fun n t rt b : err (definition typ (block typ * list (block typ))) :=
-    state <- build_expr b t ;;
+  Definition compile_fun n t rt b : cerr (definition typ (block typ * list (block typ))) :=
+    ret_blk <- incBlockNamed "Return" ;;
+    '(result, _, body) <- compile_expr b ret_blk ;;
+    body' <- body_non_empty_cast (body ++ [{|
+      blk_id    := ret_blk ;
+      blk_phis  := [];
+      blk_code  := [];
+      blk_term  := TERM_Ret result;
+      blk_comments := None
+    |}]) ;;
     ret {|
       df_prototype := {|
         dc_name := Name n
@@ -238,16 +242,19 @@ Section Compiler.
       ; dc_section := None
       ; dc_align := None
       ; dc_gc := None|}
-    ; df_args := [(Name "a_0")]
-    ; df_instrs := (entry state, rev (blocks state))
+    ; df_args := [(Name "a0")]
+    ; df_instrs := body'
     |}.
 
   Definition compile_def (d : def) : err (toplevel_entity typ (block typ * list (block typ))) :=
     match d with
-    | FunDef n t rt b => TLE_Definition <$> compile_fun n t rt b
+    | FunDef n t rt b => evalErrS (TLE_Definition <$> compile_fun n t rt b) (start_state (compile_type t))
     end.
 
   Definition compile_cogent : cogent_prog -> err (toplevel_entities typ (block typ * list (block typ))) :=
     map_monad compile_def.
+
+  (* Definition compile_cogent (e : expr) := compile_expr e (Name "exit") (newState (TYPE_I 8)). *)
+  
 
 End Compiler.
