cogent/llvm/checker/coq/Corres.v
@@ -5,22 +5,21 @@ From ITree Require Import ITree ITreeFacts.
 From Vellvm Require Import LLVMAst LLVMEvents TopLevel Handlers InterpreterMCFG TopLevelRefinements DynamicTypes
   CFG TypToDtyp InterpretationStack.
 
-From Checker Require Import Denote Cogent Compiler Utils.Fail.
+From Checker Require Import Denote Cogent Compiler Utils.Codegen Utils.Fail.
 
 Import ListNotations.
-
 
 Definition vellvm_prog : Type := toplevel_entities typ (block typ * list (block typ)).
 
 (* Lifted from Helix *)
-Definition E_mcfg : Type -> Type := (ExternalCallE +' PickE +' UBE +' DebugE +' FailureE).
-(* Definition E_cfg : Type -> Type := (CallE +' PickE +' UBE +' DebugE +' FailureE).  *)
+Definition E_mcfg : Type -> Type := ExternalCallE +' PickE +' UBE +' DebugE +' FailureE.
+Definition E_cfg : Type -> Type := CallE +' PickE +' UBE +' DebugE +' FailureE. 
 Definition semantics_llvm_mcfg p : itree E_mcfg _ := model_to_L3 DTYPE_Void "main" [DV.UVALUE_I32 (DynamicValues.Int32.zero)] p.
 Definition semantics_llvm (p : vellvm_prog) : itree E_mcfg _ :=
   semantics_llvm_mcfg (convert_types (mcfg_of_tle p)).
 
 Definition semantics_cogent (p : cogent_prog) : failT (itree E_mcfg) (memory * uval) := 
-  interp_cogent (prog_to_module p) (UFunction "main") UUnit dummy_memory.
+  interp_cogent (denote_program p) "main" UUnit dummy_memory.
 
 Section TopLevel.
 
@@ -29,7 +28,8 @@ Section TopLevel.
 
   Lemma compiler_correct :
     forall (c : cogent_prog) (ll : vellvm_prog),
-      compile_cogent c = inr ll -> eutt TT (semantics_cogent c) (semantics_llvm ll).
+      compile_cogent c = inr ll ->
+        eutt TT (semantics_cogent c) (semantics_llvm ll).
   Proof.
   Abort.
 
@@ -37,35 +37,19 @@ End TopLevel.
 
 Section Expressions.
 
-(* we want something like Lemma genNExpr_correct *)
+  Lemma compile_expr_correct :
+    forall (s1 s2 : CodegenState) (v : texp typ)
+           (e : expr) (γ : ctx) (cogent_mem : memory)
+           (next_blk blk prev_blk : block_id) (blks : ocfg typ)
+           (g : global_env) (l : local_env) (vellvm_mem : memory_stack),
+      compile_expr e next_blk s1 = inr (s2, (v, blk, blks)) ->
+        eutt
+          TT
+          (interp_expr (denote_expr γ e) cogent_mem)
+          (interp_cfg3 (denote_ocfg (convert_typ [] blks) (prev_blk, next_blk)) g l vellvm_mem).
+  Proof.
+  Abort.
+
+(* we want something like Lemma genNExpr_correct mixed with DSHAssign_correct *)
 
 End Expressions.
-
-(* Definition vellvm_env : Type := memory_stack * (local_env * global_env).
-Definition interp_vellvm (t : itree L0 uvalue) (e : vellvm_env) : itree L3 res_L3 :=
-  interp_mcfg3 t (snd (snd e)) (fst (snd e), []) (fst e).
-
-Definition relate_env (c_env : locals) (v_env : vellvm_env) : Prop := True. *)
-
-(* Section RAB.
-
-  Context {A B : Type}.
-  Context (RAB : A -> B -> Prop).
-
-  Definition  state_invariant (a : locals * A) (b : vellvm_env * B) : Prop := 
-    relate_env (fst a) (fst b) /\ (RAB (snd a) (snd b)).
-
-  Definition bisimilar {E} (t1 : itree (VarE +' E) A) (t2 : itree E_mcfg B) := 
-    forall c_env v_env,
-      relate_env c_env v_env ->
-        eutt state_invariant (interp_cogent t1 c_env) (interp_vellvm t2 v_env).
-
-End RAB.
-
-Definition TT {A B} : A -> B -> Prop  := fun _ _ => True.
-Hint Unfold TT : core.
-
-Definition equivalent (c : cogent_prog) (l : vellvm_prog) : Prop :=
-   bisimilar TT (denote_cogent c) (denote_vellvm l).
-
-Theorem compile_correct (c : cogent_prog) : equivalent c (compile_cogent c). *)
