cogent/llvm/checker/coq/Utils/Codegen.v
@@ -1,0 +1,155 @@
+From Coq Require Import List ZArith String.
+
+From ExtLib Require Import Structures.Monads.
+
+From Vellvm Require Import LLVMAst Util Utils.Error.
+
+From Checker Require Import Utils.ErrorWithState.
+
+Import ListNotations.
+Import MonadNotation.
+
+Local Open Scope monad_scope.
+
+Section HelixInspired.
+
+  Notation "x @@ y" := (String.append x y) (right associativity, at level 60) : string_scope.
+
+  Record CodegenState :=
+    mkCodegenState
+      {
+        block_count : nat ;
+        local_count : nat ;
+        void_count : nat ;
+        Γ : list (texp typ)
+      }.
+
+  Definition cerr := errS CodegenState.
+
+  (* Definition setVars (s : CodegenState) (newvars : list (texp typ)) : CodegenState :=
+    {|
+      block_count := block_count s ;
+      local_count := local_count s ;
+      void_count  := void_count s ;
+      Γ := newvars
+    |}. *)
+
+  (* Returns n-th varable from state or error if [n] index oob *)
+  Definition getStateVar (msg : string) (n : nat) : cerr (texp typ) :=
+    st <- get ;;
+    option2errS msg (List.nth_error (Γ st) n).
+
+  (* Definition evalCErrS {St : Type} {A : Type} (c : errS St A) (initial : St) : cerr A :=
+    match c initial with
+    | inl msg => raise msg
+    | inr (s,v) => ret v
+    end. *)
+
+  (* Definition add_comments (b : block typ) (xs : list string) : block typ :=
+    {|
+      blk_id    := blk_id b;
+      blk_phis  := blk_phis b;
+      blk_code  := blk_code b;
+      blk_term  := blk_term b;
+      blk_comments := match blk_comments b with
+                      | None => Some xs
+                      | Some ys => Some (ys++xs)
+                      end
+    |}. *)
+
+  (* Definition add_comment (bs : list (block typ)) (xs : list string) : list (block typ) :=
+    match bs with
+    | nil => nil
+    | b::bs => (add_comments b xs)::bs
+    end. *)
+
+  Definition incBlockNamed (prefix : string) : (cerr block_id) :=
+    st <- get  ;;
+    put
+      {|
+        block_count := S (block_count st);
+        local_count := local_count st ;
+        void_count := void_count st ;
+        Γ := Γ st
+      |} ;;
+    ret (Name (prefix ++ string_of_nat (block_count st))).
+
+  (* Definition incBlock := incBlockNamed "b". *)
+
+  Definition incLocalNamed (prefix : string) : (cerr raw_id) :=
+    st <- get ;;
+    put
+      {|
+        block_count := block_count st ;
+        local_count := S (local_count st) ;
+        void_count  := void_count st ;
+        Γ := Γ st
+      |} ;;
+    ret (Name (prefix @@ string_of_nat (local_count st))).
+
+  Definition incLocal := incLocalNamed "l".
+
+  Definition incVoid : (cerr int) :=
+    st <- get ;;
+    put
+      {|
+        block_count := block_count st ;
+        local_count := local_count st ;
+        void_count  := S (void_count st) ;
+        Γ := Γ st
+      |} ;;
+    ret (Z.of_nat (void_count st)).
+
+  Definition addVars (newvars : list (texp typ)) : cerr unit :=
+    st <- get ;;
+    put
+      {|
+        block_count := block_count st ;
+        local_count := local_count st ;
+        void_count  := void_count st ;
+        Γ := newvars ++ Γ st
+      |}.
+
+  Fixpoint drop_err {A : Type} (n : nat) (lst : list A) : err (list A)
+    := match n, lst with
+      | O, xs => ret xs
+      | S n', (_::xs) => drop_err n' xs
+      | _, _ => raise "drop on empty list"
+      end.
+
+  Definition dropVars (n : nat) : cerr unit :=
+    st <- get ;;
+    Γ' <- err2errS (drop_err n (Γ st)) ;;
+    put {|
+        block_count := block_count st ;
+        local_count := local_count st ;
+        void_count  := void_count st ;
+        Γ := Γ'
+      |}.
+
+  Definition body_non_empty_cast (body : list (block typ)) : cerr (block typ * list (block typ)) :=
+    match body with
+    | [] => raise "Attempting to generate a function containing no block"
+    | b::body => ret (b,body)
+    end.
+
+End HelixInspired.
+
+Section AdditionalHelpers.
+
+  Definition code_block (id next : block_id) (c : code typ) : block typ := {|
+    blk_id    := id ;
+    blk_phis  := [];
+    blk_code  := c;
+    blk_term  := TERM_Br_1 next;
+    blk_comments := None
+  |}.
+
+  Definition start_state (t : typ) : CodegenState := {|
+    block_count := 0 ;
+    local_count := 0 ;
+    void_count  := 0 ;
+    Γ := [(t, EXP_Ident (ID_Local (Name "a0")))]
+  |}.
+
+End AdditionalHelpers.
